Substore, partial store

Common.v
@@ -3,8 +3,27 @@ From Coq Require Import ZArith Lia Bool List String Program.Equality.
 Local Open Scope Z_scope.
 
 Local Open Scope string_scope.
-  Definition ident := string.
-  Definition store : Type := ident -> Z.
-  Definition sempty : store := (fun _ => 0).
-  Definition supdate (x: ident) (v: Z) (s: store) : store :=
-    fun y => if string_dec x y then v else s y.
+
+Definition ident := string.
+Definition store : Type := ident -> option Z.
+Definition sempty : store := (fun _ => None).
+Definition supdate (x: ident) (v: Z) (s: store) : store :=
+  fun y => if string_dec x y then Some v else s y.
+
+Lemma supdate_same: forall l v h, (supdate l v h) l = Some v.
+Proof.
+  intros; cbn.
+  unfold supdate.
+  destruct (string_dec l l); congruence.
+Qed.
+
+Lemma supdate_other: forall l v h l', l <> l' -> (supdate l v h) l' = h l'.
+Proof.
+  intros; cbn.
+  unfold supdate.
+  destruct (string_dec l l'); congruence.
+Qed.
+
+(* s1 <= s2 *)
+Definition substore (s1 s2 : store) :=
+  forall v x, s1 x = Some v -> s2 x = Some v.
